src/Memory2.v
@@ -1,0 +1,53 @@
+From Coq Require Import
+     Arith.PeanoNat
+     Logic.FunctionalExtensionality.
+
+Require Export Heapster.Permissions.
+
+(* Memory model *)
+Definition block := nat.
+Definition offset := nat.
+Definition addr : Set := block * offset.
+
+Definition eqb (a b : addr) : bool :=
+  Nat.eqb (fst a) (fst b) && Nat.eqb (snd a) (snd b).
+
+Lemma addr_dec : forall (a b : addr), {a = b} + {a <> b}.
+Proof.
+  intros [a1 a2] [b1 b2].
+  destruct (Nat.eq_dec a1 b1); destruct (Nat.eq_dec a2 b2); subst; auto.
+  - right. intros H. inversion H; subst. apply n. reflexivity.
+  - right. intros H. inversion H; subst. apply n. reflexivity.
+  - right. intros H. inversion H; subst. apply n. reflexivity.
+Qed.
+
+Lemma addr_neq_cases (b b' o o' : nat) :
+  (b, o) <> (b', o') -> b <> b' \/ o <> o'.
+Proof.
+  intros.
+  destruct (Nat.eq_dec b b'); destruct (Nat.eq_dec o o'); subst; auto.
+Qed.
+
+Lemma eqb_spec : forall x y, Bool.reflect (x = y) (eqb x y).
+Proof.
+  intros [x1 x2] [y1 y2]. destruct (eqb (x1, x2) (y1, y2)) eqn:?; constructor.
+  - unfold eqb in Heqb. simpl in Heqb. symmetry in Heqb. apply Bool.andb_true_eq in Heqb.
+    destruct Heqb. symmetry in H, H0.
+    apply (Bool.reflect_iff _ _ (Nat.eqb_spec _ _)) in H.
+    apply (Bool.reflect_iff _ _ (Nat.eqb_spec _ _)) in H0. subst. auto.
+  - unfold eqb in Heqb. simpl in Heqb. apply Bool.andb_false_iff in Heqb.
+    destruct Heqb.
+    + intro. inversion H0. subst. rewrite Nat.eqb_refl in H. inversion H.
+    + intro. inversion H0. subst. rewrite Nat.eqb_refl in H. inversion H.
+Qed.
+
+Inductive Value :=
+| VNum : nat -> Value
+| VPtr : addr -> Value
+.
+Definition mem_block := offset -> option Value.
+
+Variant logical_block :=
+| LBlock (size : offset) (bytes : mem_block) : logical_block.
+
+Definition memory := list (option logical_block).
